save all changes

third_party/move/documentation/tutorial/step_1/BasicCoin/sources/FirstModule.move
@@ -1,44 +1,13 @@
-module 0x82::Test {
-    struct R has key {
-        x: u64,
+module 0x42::Test {
+    struct R has key{
+        v1: u64,
+        v2: u64
     }
-    struct Y has key {
-        x: u64,
-    }
-
     spec module {
-        invariant forall a: address where exists<R>(a):
-            a == @0x0;
-        invariant forall b: address where exists<Y>(b):
-            b == @0x30;
-        invariant forall a: address where exists<R>(a):
-            forall b: address where exists<Y>(b):
-                global<R>(a).x >= global<Y>(b).x;
+        invariant update forall addr: address where old(exists<R>(addr)): exists<R>(addr);
     }
-
-    public fun incr(a: address, b:address) acquires R, Y{
-        let r = borrow_global_mut<R>(a);
-        r.x = r.x + 1;
-        //write back to R happense here
-        //Invariant Checks injected here
-
-        let r2 = borrow_global_mut<Y>(b);
-        r2.x = r2.x + 1;
-        //write back to Y happense here
-        //Invariant Checks injected here
-    }
-    public fun incr2(a: address, b:address) acquires R, Y{
-        let r = borrow_global_mut<R>(a);
-        let r2 = borrow_global_mut<Y>(b);
-        r.x = r.x + 1;
-        //write back to R happense here
-        //Invariant injected here
-        r2.x = r2.x + 1;
-    }
-    public fun incr3(a: address, b:address) acquires R, Y{
-        let r2 = borrow_global_mut<Y>(b);
-        let r = borrow_global_mut<R>(a);
-        r.x = r.x + 1;
-        r2.x = r2.x + 1;
+    fun bor(a: address, b: address, p1: bool, p2: bool) acquires R {
+        let c = if (p2) borrow_global_mut<R>(a) else borrow_global_mut<R>(a);
+        c.v1 = c.v1+1;
     }
 }
