third_party/move/documentation/tutorial/step_2/BasicCoin/sources/FirstModule.move
@@ -1,18 +1,27 @@
 module 0x82::Test {
     struct R has key {
         x: u64,
+        y: u64,
+    }
+    struct S has key {
+        x: u64,
+        y: u64,
     }
     struct Y has key {
         x: u64,
     }
 
     spec module {
-        invariant update forall a: address where exists<R>(a):
-                global<R>(a).x == old(global<R>(a).x) + 1;
+        invariant update forall a: address where old(exists<R>(a)):
+                global<R>(a).x >= old(global<R>(a).x);
+        invariant update forall a: address where old(exists<S>(a)):
+                global<S>(a).y > old(global<S>(a).y);
     }
 
-    public fun incr(a: address) acquires R{
+    public fun incr(a: address, b: address, c: bool) acquires R, S{
         let r = borrow_global_mut<R>(a);
+        let r2 = borrow_global_mut<S>(b);
         r.x = r.x + 1;
+        r2.y = r2.y+1;
     }
 }
