third_party/move/documentation/tutorial/step_1/BasicCoin/output.bpl
@@ -1112,12 +1112,17 @@ datatype $Location {
 // are single threaded in Move, we can keep them together and treat them as a value
 // during mutation until the point they are stored back to their original location.
 datatype $Mutation<T> {
-    $Mutation(l: $Location, p: Vec int, v: T, v_final: T)
+    $Mutation(l: $Location, p: Vec int, v: T, v_final: T, r_order: int, r_token: int)
 }
 
 // Representation of memory for a given type.
+
 datatype $Memory<T> {
     $Memory(domain: [int]bool, contents: [int]T)
+}
+
+datatype $MemoryPair<T> {
+    $MemoryPair(prev: $Memory T, curr: $Memory T, times: [int]int)
 }
 
 function {:builtin "MapConst"} $ConstMemoryDomain(v: bool): [int]bool;
@@ -1127,8 +1132,10 @@ axiom $ConstMemoryDomain(true) == (lambda i: int :: true);
 
 procedure $MutationAlt<T>(l: $Location, p: Vec int, v: T) returns (result: $Mutation T) {
     var prophecy: T;
+    var r_order: int;
     havoc prophecy;
-    result := $Mutation(l, p, v, prophecy);
+    havoc r_order;
+    result := $Mutation(l, p, v, prophecy, 1, 1);
     assume result->l == l;
     assume result->p == p;
     assume result->v == v;
@@ -1146,25 +1153,61 @@ function {:inline} $DereferenceProphecy<T>(ref: $Mutation T): T {
 
 // Update the value of a mutation.
 function {:inline} $UpdateMutation<T>(m: $Mutation T, v: T): $Mutation T {
-    $Mutation(m->l, m->p, v, m->v_final)
+    $Mutation(m->l, m->p, v, m->v_final, m->r_order, m->r_token)
 }
-
+function {:inline} $UpdateMutationRToken<T1, T2>(m: $Mutation T1, mc: $Mutation T2): $Mutation T1 {
+    $Mutation(m->l, m->p, m->v, m->v_final, m->r_order, m->r_token - mc->r_token)
+}
 //prophecy Fullfilled
-function {:inline} $Fulfilled<T>(ref: $Mutation T): bool {
-    ref->v == ref->v_final
+
+var $asserts_results: int;
+//For a flow that does not existe:
+//If assert passed, then there's going to be a future assert that fails it
+//If assert failed, then we store both the message
+//The location of write_back is not fixed now. So location of assert is also not fixed.
+var $assertType: int;
+var $asserts_time: int;
+//For global/function/struct invariant injected
+// 2 ways to approach this:
+//1. pass the global states back?? Then have checks happen at time of borrow
+// - additional 2 havoc varibles: before states and after states.
+// global[order-1] and global[order]
+// for each invidivdual value if cur_index > order then return old,
+// if cur_index <= order then return new.
+// assert fail do not result in failure immediately
+//2. Record down all updates, then check at the end? How do I know I hit end though?
+// - explicite entry point functions and explicite inline functions.
+//
+//euler's tour on the borrow graph
+//pass it down the right most edges
+//For loop invariant specified in body
+//ToDo: do the checks at place of borrow with prophecied states. But
+//don't assert, just save result to global var
+//Then at r_order th write back, assume the state to current states.
+//update current states at each write back?
+//assert at very end.
+function {:inline} $Fulfilled<T>(ref: $Mutation T, c_index: int): bool {
+    ref->v == ref->v_final &&
+    ((ref->r_token > 0 && c_index == ref->r_order) ||
+    (ref->r_token == 0 && c_index >= ref->r_order))
 }
 
 function {:inline} $ChildMutation<T1, T2>(m: $Mutation T1, offset: int, v: T2): $Mutation T2 {
-    $Mutation(m->l, ExtendVec(m->p, offset), v, v)
+    $Mutation(m->l, ExtendVec(m->p, offset), v, v, m->r_order, m->r_token)
 }
 //functions are pure and deterministic, have to use procedure
+
 procedure $ChildMutationAlt<T1, T2>(m: $Mutation T1, offset: int, v: T2) returns (result: $Mutation T2) {
     var prophecy: T2;
+    var r_token: int;
     havoc prophecy;
-    result := $Mutation(m->l, ExtendVec(m->p, offset), v, prophecy);
+    havoc r_token;
+    result := $Mutation(m->l, ExtendVec(m->p, offset), v, prophecy, m->r_order, r_token);
     assume result->l == m->l;
     assume result->p == ExtendVec(m->p, offset);
     assume result->v == v;
+    assume r_token >= 0 && r_token <= m->r_token;
+    //if you have the token, you may pass it down.
 }
 
 // Return true if two mutations share the location and path
@@ -1229,20 +1272,52 @@ function {:inline} $GlobalLocationAddress<T>(m: $Mutation T): int {
 function {:inline} $ResourceExists<T>(m: $Memory T, addr: int): bool {
     m->domain[addr]
 }
+//individual timestamp for all address
+function {:inline} $ResourceExistsMP<T>(mp: $MemoryPair T, addr: int, c_index: int): bool {
+    if c_index >= mp->times[addr] then
+        mp->curr->domain[addr]
+    else
+        mp->prev->domain[addr]
+}
 
 // Obtains Value of given resource.
 function {:inline} $ResourceValue<T>(m: $Memory T, addr: int): T {
     m->contents[addr]
 }
 
+function {:inline} $ResourceValueMP<T>(mp: $MemoryPair T, addr: int, c_index: int): T {
+    if c_index >= mp->times[addr] then
+        mp->curr->contents[addr]
+    else
+        mp->prev->contents[addr]
+}
+
 // Update resource.
 function {:inline} $ResourceUpdate<T>(m: $Memory T, a: int, v: T): $Memory T {
     $Memory(m->domain[a := true], m->contents[a := v])
+}
+function {:inline} $ResourceUpdateMP<T>(mp: $MemoryPair T, a: int, v: T, proph_index: int): $MemoryPair T {
+    $MemoryPair(
+        // old: gets domain and value from new for this address
+        $Memory(mp->prev->domain[a:= mp->curr->domain[a]], mp->prev->contents[a:= mp->curr->contents[a]]),
+        $Memory(mp->curr->domain[a:= true], mp->curr->contents[a:= v]),
+        //update times
+        mp->times[a := proph_index]
+    )
 }
 
 // Remove resource.
 function {:inline} $ResourceRemove<T>(m: $Memory T, a: int): $Memory T {
     $Memory(m->domain[a := false], m->contents)
+}
+
+function {:inline} $ResourceRemoveMP<T>(mp: $MemoryPair T, a: int, proph_index: int): $MemoryPair T {
+    $MemoryPair(
+        $Memory(mp->prev->domain[a := mp->curr->domain[a]], mp->prev->contents[a:= mp->curr->contents[a]]),
+        $Memory(mp->curr->domain[a := false], mp->curr->contents),
+        //update times
+        mp->times[a := proph_index]
+    )
 }
 
 // Copies resource from memory s to m.
@@ -1251,6 +1326,15 @@ function {:inline} $ResourceCopy<T>(m: $Memory T, s: $Memory T, a: int): $Memory
             m->contents[a := s->contents[a]])
 }
 
+function {:inline} $ResourceCopyMP<T>(m: $MemoryPair T, s: $MemoryPair T, a: int, c_index: int): $MemoryPair T {
+    $MemoryPair(
+    $Memory(m->prev->domain[a := s->curr->domain[a]],
+            m->prev->contents[a := s->curr->contents[a]]),
+    $Memory(m->curr->domain[a := $ResourceExistsMP(s, a, c_index)],
+            m->curr->contents[a := $ResourceValueMP(s, a, c_index)]),
+    m->times
+    )
+}
 
 
 // ============================================================================================
@@ -1282,13 +1366,24 @@ procedure {:inline 1} $Abort(code: int) {
 function {:inline} $StdError(cat: int, reason: int): int {
     reason * 256 + cat
 }
+var $cur_index: int; //default is initialized to 0
+var $cur_index_initialized: bool;
 
-procedure {:inline 1} $InitVerification() {
+procedure {:inline 1} $InitVerification() returns (isEntryPoint: bool) {
     // Set abort_flag to false, and havoc abort_code
+    // returns whether the current function is entry point function.
     $abort_flag := false;
     havoc $abort_code;
     // Initialize event store
     call $InitEventStore();
+    if (!$cur_index_initialized){
+        $cur_index := 0;
+        $cur_index_initialized := true;
+        isEntryPoint := true;
+    }
+    else{
+        isEntryPoint := false;
+    }
 }
 
 // ============================================================================================
@@ -3265,7 +3360,7 @@ returns (dst: $Mutation (int), m': $Mutation (Vec (int)))
 
     call dst := $MutationAlt(m->l, ExtendVec(m->p, index), ReadVec(v, index));
     assume dst->l == m->l;
-    assume dst->p == m->p;
+    assume dst->p == ExtendVec(m->p, index);
     assume dst->v == ReadVec(v, index);
     m' := $UpdateMutation(m, UpdateVec(v, index, $DereferenceProphecy(dst)));
 
@@ -3532,671 +3627,309 @@ datatype $TypeParamInfo {
 // Given Types for Type Parameters
 
 
-// struct Test::R at ./sources/FirstModule.move:2:5+40
-datatype $82_Test_R {
-    $82_Test_R($x: int)
+// struct Test::R at ./sources/FirstModule.move:2:5+56
+datatype $42_Test_R {
+    $42_Test_R($v1: int, $v2: int)
 }
-function {:inline} $Update'$82_Test_R'_x(s: $82_Test_R, x: int): $82_Test_R {
-    $82_Test_R(x)
+function {:inline} $Update'$42_Test_R'_v1(s: $42_Test_R, x: int): $42_Test_R {
+    $42_Test_R(x, s->$v2)
 }
-function $IsValid'$82_Test_R'(s: $82_Test_R): bool {
-    $IsValid'u64'(s->$x)
+function {:inline} $Update'$42_Test_R'_v2(s: $42_Test_R, x: int): $42_Test_R {
+    $42_Test_R(s->$v1, x)
 }
-function {:inline} $IsEqual'$82_Test_R'(s1: $82_Test_R, s2: $82_Test_R): bool {
+function $IsValid'$42_Test_R'(s: $42_Test_R): bool {
+    $IsValid'u64'(s->$v1)
+      && $IsValid'u64'(s->$v2)
+}
+function {:inline} $IsEqual'$42_Test_R'(s1: $42_Test_R, s2: $42_Test_R): bool {
     s1 == s2
 }
-var $82_Test_R_$memory: $Memory $82_Test_R;
-
-// struct Test::Y at ./sources/FirstModule.move:5:5+40
-datatype $82_Test_Y {
-    $82_Test_Y($x: int)
-}
-function {:inline} $Update'$82_Test_Y'_x(s: $82_Test_Y, x: int): $82_Test_Y {
-    $82_Test_Y(x)
-}
-function $IsValid'$82_Test_Y'(s: $82_Test_Y): bool {
-    $IsValid'u64'(s->$x)
-}
-function {:inline} $IsEqual'$82_Test_Y'(s1: $82_Test_Y, s2: $82_Test_Y): bool {
-    s1 == s2
-}
-var $82_Test_Y_$memory: $Memory $82_Test_Y;
-
-// fun Test::incr [verification] at ./sources/FirstModule.move:19:5+353
-procedure {:timeLimit 80} $82_Test_incr$verify(_$t0: int, _$t1: int) returns ()
+var $42_Test_R_$memory: $Memory $42_Test_R;
+var $42_Test_R_$memoryPair: $MemoryPair $42_Test_R;
+// fun Test::bor [verification] at ./sources/FirstModule.move:9:5+171
+procedure {:timeLimit 80} $42_Test_bor$verify(_$t0: int, _$t1: int, _$t2: bool, _$t3: bool) returns ()
 {
     // declare local variables
-    var $t2: $Mutation ($82_Test_R);
-    var $t3: $Mutation ($82_Test_Y);
-    var $t4: $Mutation ($82_Test_R);
-    var $t5: int;
-    var $t6: int;
-    var $t7: int;
+    var $isEntryPoint: bool;
+    var $t4: $Mutation ($42_Test_R);
+    var $t5: $Mutation ($42_Test_R);
+    var $t6: $Mutation ($42_Test_R);
+    var $t7: $Mutation ($42_Test_R);
     var $t8: int;
-    var $t9: $Mutation (int);
-    var $t10: $Mutation ($82_Test_Y);
+    var $t9: int;
+    var $t10: int;
     var $t11: int;
-    var $t12: int;
-    var $t13: int;
-    var $t14: $Mutation (int);
+    var $t12: $Mutation (int);
     var $t0: int;
     var $t1: int;
-    var $temp_0'$82_Test_R': $82_Test_R;
-    var $temp_0'$82_Test_Y': $82_Test_Y;
+    var $t2: bool;
+    var $t3: bool;
+    var $temp_0'$42_Test_R': $42_Test_R;
     var $temp_0'address': int;
+    var $temp_0'bool': bool;
+    var $42_Test_R_$memory#1: $Memory $42_Test_R;
+    var $42_Test_R_$memory#2: $Memory $42_Test_R;
+    var $tempresult: bool;
     $t0 := _$t0;
     $t1 := _$t1;
+    $t2 := _$t2;
+    $t3 := _$t3;
 
     // verification entrypoint assumptions
-    call $InitVerification();
+    call $isEntryPoint := $InitVerification();
 
     // bytecode translation starts here
-    // assume WellFormed($t0) at ./sources/FirstModule.move:19:5+1
-    assume {:print "$at(2,455,456)"} true;
+    // assume WellFormed($t0) at ./sources/FirstModule.move:9:5+1
+    assume {:print "$at(2,200,201)"} true;
     assume $IsValid'address'($t0);
 
-    // assume WellFormed($t1) at ./sources/FirstModule.move:19:5+1
+    // assume WellFormed($t1) at ./sources/FirstModule.move:9:5+1
     assume $IsValid'address'($t1);
 
-    // assume forall $rsc: Test::R: ResourceDomain<Test::R>(): WellFormed($rsc) at ./sources/FirstModule.move:19:5+1
-    assume (forall $a_0: int :: {$ResourceValue($82_Test_R_$memory, $a_0)}(var $rsc := $ResourceValue($82_Test_R_$memory, $a_0);
-    ($IsValid'$82_Test_R'($rsc))));
+    // assume WellFormed($t2) at ./sources/FirstModule.move:9:5+1
+    assume $IsValid'bool'($t2);
 
-    // assume forall $rsc: Test::Y: ResourceDomain<Test::Y>(): WellFormed($rsc) at ./sources/FirstModule.move:19:5+1
-    assume (forall $a_0: int :: {$ResourceValue($82_Test_Y_$memory, $a_0)}(var $rsc := $ResourceValue($82_Test_Y_$memory, $a_0);
-    ($IsValid'$82_Test_Y'($rsc))));
+    // assume WellFormed($t3) at ./sources/FirstModule.move:9:5+1
+    assume $IsValid'bool'($t3);
 
-    // assume forall a: address: TypeDomain<address>() where exists<Test::R>(a): Eq<address>(a, 0x0) at ./sources/FirstModule.move:19:5+353
-    // global invariant at ./sources/FirstModule.move:10:9+70
-    assume (forall a: int :: $IsValid'address'(a) ==> ($ResourceExists($82_Test_R_$memory, a))  ==> ($IsEqual'address'(a, 0)));
+    // assume forall $rsc: Test::R: ResourceDomain<Test::R>(): WellFormed($rsc) at ./sources/FirstModule.move:9:5+1
+    assume (forall $a_0: int :: {$ResourceValue($42_Test_R_$memory, $a_0)}(var $rsc := $ResourceValue($42_Test_R_$memory, $a_0);
+    ($IsValid'$42_Test_R'($rsc))));
 
-    // assume forall b: address: TypeDomain<address>() where exists<Test::Y>(b): Eq<address>(b, 0x30) at ./sources/FirstModule.move:19:5+353
-    // global invariant at ./sources/FirstModule.move:12:9+71
-    assume (forall b: int :: $IsValid'address'(b) ==> ($ResourceExists($82_Test_Y_$memory, b))  ==> ($IsEqual'address'(b, 48)));
+    $42_Test_R_$memoryPair := $MemoryPair($42_Test_R_$memory, $42_Test_R_$memory, 0);
 
-    // assume forall a: address: TypeDomain<address>() where exists<Test::R>(a): forall b: address: TypeDomain<address>() where exists<Test::Y>(b): Ge(select Test::R.x<Test::R>(global<Test::R>(a)), select Test::Y.x<Test::Y>(global<Test::Y>(b))) at ./sources/FirstModule.move:19:5+353
-    // global invariant at ./sources/FirstModule.move:14:9+147
-    assume (forall a: int :: $IsValid'address'(a) ==> ($ResourceExists($82_Test_R_$memory, a))  ==> ((forall b: int :: $IsValid'address'(b) ==> ($ResourceExists($82_Test_Y_$memory, b))  ==> (($ResourceValue($82_Test_R_$memory, a)->$x >= $ResourceValue($82_Test_Y_$memory, b)->$x)))));
+    // uninit($t6) at <internal>:1:1+10
+    assume {:print "$at(1,0,10)"} true;
+    assume $t6->l == $Uninitialized();
 
-    // trace_local[a]($t0) at ./sources/FirstModule.move:19:5+1
+    // uninit($t7) at <internal>:1:1+10
+    assume $t7->l == $Uninitialized();
+
+    // trace_local[a]($t0) at ./sources/FirstModule.move:9:5+1
+    assume {:print "$at(2,200,201)"} true;
     assume {:print "$track_local(1,0,0):", $t0} $t0 == $t0;
 
-    // trace_local[b]($t1) at ./sources/FirstModule.move:19:5+1
+    // trace_local[b]($t1) at ./sources/FirstModule.move:9:5+1
     assume {:print "$track_local(1,0,1):", $t1} $t1 == $t1;
 
-    // $t4 := borrow_global<Test::R>($t0) on_abort goto L2 with $t5 at ./sources/FirstModule.move:20:17+17
-    assume {:print "$at(2,525,542)"} true;
-    if (!$ResourceExists($82_Test_R_$memory, $t0)) {
-        call $ExecFailureAbort();
-    } else {
-        call $t4 := $MutationAlt($Global($t0), EmptyVec(), $ResourceValue($82_Test_R_$memory, $t0));
-        assume $ResourceValue($82_Test_R_$memory, $t0) == $Dereference($t4);
-        $82_Test_R_$memory := $ResourceUpdate($82_Test_R_$memory, $t0, $DereferenceProphecy($t4));
-    }
-    if ($abort_flag) {
-        assume {:print "$at(2,525,542)"} true;
-        $t5 := $abort_code;
-        assume {:print "$track_abort(1,0):", $t5} $t5 == $t5;
-        goto L2;
-    }
+    // trace_local[p1]($t2) at ./sources/FirstModule.move:9:5+1
+    assume {:print "$track_local(1,0,2):", $t2} $t2 == $t2;
 
-    // trace_local[r]($t4) at ./sources/FirstModule.move:20:13+1
-    $temp_0'$82_Test_R' := $Dereference($t4);
-    assume {:print "$track_local(1,0,2):", $temp_0'$82_Test_R'} $temp_0'$82_Test_R' == $temp_0'$82_Test_R';
+    // trace_local[p2]($t3) at ./sources/FirstModule.move:9:5+1
+    assume {:print "$track_local(1,0,3):", $t3} $t3 == $t3;
 
-    // $t6 := get_field<Test::R>.x($t4) at ./sources/FirstModule.move:21:15+3
-    assume {:print "$at(2,564,567)"} true;
-    $t6 := $Dereference($t4)->$x;
+    // if ($t3) goto L5 else goto L6 at ./sources/FirstModule.move:10:17+60
+    assume {:print "$at(2,281,341)"} true;
+    if ($t3) { goto L5; } else { goto L6; }
 
-    // $t7 := 1 at ./sources/FirstModule.move:21:21+1
-    $t7 := 1;
-    assume $IsValid'u64'($t7);
-
-    // $t8 := +($t6, $t7) on_abort goto L2 with $t5 at ./sources/FirstModule.move:21:19+1
-    call $t8 := $AddU64($t6, $t7);
-    if ($abort_flag) {
-        assume {:print "$at(2,568,569)"} true;
-        $t5 := $abort_code;
-        assume {:print "$track_abort(1,0):", $t5} $t5 == $t5;
-        goto L2;
-    }
-
-    // $t9 := borrow_field<Test::R>.x($t4) at ./sources/FirstModule.move:21:9+3
-    call $t9 := $ChildMutationAlt($t4, 0, $Dereference($t4)->$x);
-    assume $Dereference($t9) == $Dereference($t4)->$x;
-    $t4 := $UpdateMutation($t4, $Update'$82_Test_R'_x($Dereference($t4), $DereferenceProphecy($t9)));
-
-    // fulfilled($t4) at ./sources/FirstModule.move:21:9+3
-    assume $Fulfilled($t4);
-
-    // write_ref($t9, $t8) at ./sources/FirstModule.move:21:9+13
-    $t9 := $UpdateMutation($t9, $t8);
-
-    // write_back[Reference($t4).x (u64)]($t9) at ./sources/FirstModule.move:21:9+13
-    assume $Fulfilled($t9);
-
-    // write_back[Test::R@]($t4) at ./sources/FirstModule.move:21:9+13
-    assume $Dereference($t4) == $DereferenceProphecy($t4);
-
-    // assert forall a: address: TypeDomain<address>() where exists<Test::R>(a): Eq<address>(a, 0x0) at ./sources/FirstModule.move:10:9+70
-    // global invariant at ./sources/FirstModule.move:10:9+70
-    assume {:print "$at(2,137,207)"} true;
-    assert {:msg "assert_failed(2,137,207): global memory invariant does not hold"}
-      (forall a: int :: $IsValid'address'(a) ==> ($ResourceExists($82_Test_R_$memory, a))  ==> ($IsEqual'address'(a, 0)));
-
-    // assert forall a: address: TypeDomain<address>() where exists<Test::R>(a): forall b: address: TypeDomain<address>() where exists<Test::Y>(b): Ge(select Test::R.x<Test::R>(global<Test::R>(a)), select Test::Y.x<Test::Y>(global<Test::Y>(b))) at ./sources/FirstModule.move:14:9+147
-    // global invariant at ./sources/FirstModule.move:14:9+147
-    assume {:print "$at(2,296,443)"} true;
-    assert {:msg "assert_failed(2,296,443): global memory invariant does not hold"}
-      (forall a: int :: $IsValid'address'(a) ==> ($ResourceExists($82_Test_R_$memory, a))  ==> ((forall b: int :: $IsValid'address'(b) ==> ($ResourceExists($82_Test_Y_$memory, b))  ==> (($ResourceValue($82_Test_R_$memory, a)->$x >= $ResourceValue($82_Test_Y_$memory, b)->$x)))));
-
-    // $t10 := borrow_global<Test::Y>($t1) on_abort goto L2 with $t5 at ./sources/FirstModule.move:25:18+17
-    assume {:print "$at(2,672,689)"} true;
-    if (!$ResourceExists($82_Test_Y_$memory, $t1)) {
-        call $ExecFailureAbort();
-    } else {
-        call $t10 := $MutationAlt($Global($t1), EmptyVec(), $ResourceValue($82_Test_Y_$memory, $t1));
-        assume $ResourceValue($82_Test_Y_$memory, $t1) == $Dereference($t10);
-        $82_Test_Y_$memory := $ResourceUpdate($82_Test_Y_$memory, $t1, $DereferenceProphecy($t10));
-    }
-    if ($abort_flag) {
-        assume {:print "$at(2,672,689)"} true;
-        $t5 := $abort_code;
-        assume {:print "$track_abort(1,0):", $t5} $t5 == $t5;
-        goto L2;
-    }
-
-    // trace_local[r2]($t10) at ./sources/FirstModule.move:25:13+2
-    $temp_0'$82_Test_Y' := $Dereference($t10);
-    assume {:print "$track_local(1,0,3):", $temp_0'$82_Test_Y'} $temp_0'$82_Test_Y' == $temp_0'$82_Test_Y';
-
-    // $t11 := get_field<Test::Y>.x($t10) at ./sources/FirstModule.move:26:16+4
-    assume {:print "$at(2,712,716)"} true;
-    $t11 := $Dereference($t10)->$x;
-
-    // $t12 := 1 at ./sources/FirstModule.move:26:23+1
-    $t12 := 1;
-    assume $IsValid'u64'($t12);
-
-    // $t13 := +($t11, $t12) on_abort goto L2 with $t5 at ./sources/FirstModule.move:26:21+1
-    call $t13 := $AddU64($t11, $t12);
-    if ($abort_flag) {
-        assume {:print "$at(2,717,718)"} true;
-        $t5 := $abort_code;
-        assume {:print "$track_abort(1,0):", $t5} $t5 == $t5;
-        goto L2;
-    }
-
-    // $t14 := borrow_field<Test::Y>.x($t10) at ./sources/FirstModule.move:26:9+4
-    call $t14 := $ChildMutationAlt($t10, 0, $Dereference($t10)->$x);
-    assume $Dereference($t14) == $Dereference($t10)->$x;
-    $t10 := $UpdateMutation($t10, $Update'$82_Test_Y'_x($Dereference($t10), $DereferenceProphecy($t14)));
-
-    // fulfilled($t10) at ./sources/FirstModule.move:26:9+4
-    assume $Fulfilled($t10);
-
-    // write_ref($t14, $t13) at ./sources/FirstModule.move:26:9+15
-    $t14 := $UpdateMutation($t14, $t13);
-
-    // write_back[Reference($t10).x (u64)]($t14) at ./sources/FirstModule.move:26:9+15
-    assume $Fulfilled($t14);
-
-    // write_back[Test::Y@]($t10) at ./sources/FirstModule.move:26:9+15
-    assume $Dereference($t10) == $DereferenceProphecy($t10);
-
-    // assert forall b: address: TypeDomain<address>() where exists<Test::Y>(b): Eq<address>(b, 0x30) at ./sources/FirstModule.move:12:9+71
-    // global invariant at ./sources/FirstModule.move:12:9+71
-    assume {:print "$at(2,216,287)"} true;
-    assert {:msg "assert_failed(2,216,287): global memory invariant does not hold"}
-      (forall b: int :: $IsValid'address'(b) ==> ($ResourceExists($82_Test_Y_$memory, b))  ==> ($IsEqual'address'(b, 48)));
-
-    // assert forall a: address: TypeDomain<address>() where exists<Test::R>(a): forall b: address: TypeDomain<address>() where exists<Test::Y>(b): Ge(select Test::R.x<Test::R>(global<Test::R>(a)), select Test::Y.x<Test::Y>(global<Test::Y>(b))) at ./sources/FirstModule.move:14:9+147
-    // global invariant at ./sources/FirstModule.move:14:9+147
-    assume {:print "$at(2,296,443)"} true;
-    assert {:msg "assert_failed(2,296,443): global memory invariant does not hold"}
-      (forall a: int :: $IsValid'address'(a) ==> ($ResourceExists($82_Test_R_$memory, a))  ==> ((forall b: int :: $IsValid'address'(b) ==> ($ResourceExists($82_Test_Y_$memory, b))  ==> (($ResourceValue($82_Test_R_$memory, a)->$x >= $ResourceValue($82_Test_Y_$memory, b)->$x)))));
-
-    // label L1 at ./sources/FirstModule.move:29:5+1
-    assume {:print "$at(2,807,808)"} true;
+    // label L1 at ./sources/FirstModule.move:10:46+1
 L1:
 
-    // return () at ./sources/FirstModule.move:29:5+1
-    assume {:print "$at(2,807,808)"} true;
-    return;
+    // $t6 := borrow_global<Test::R>($t0) on_abort goto L4 with $t8 at ./sources/FirstModule.move:10:25+17
+    assume {:print "$at(2,289,306)"} true;
+    if (!$ResourceExists($42_Test_R_$memory, $t0)) {
+        call $ExecFailureAbort();
+    } else {
+        call $t6 := $MutationAlt($Global($t0), EmptyVec(), $ResourceValue($42_Test_R_$memory, $t0));
+        assume $ResourceValue($42_Test_R_$memory, $t0) == $Dereference($t6);
+        $42_Test_R_$memory#1 := $42_Test_R_$memory;
+        $42_Test_R_$memory := $ResourceUpdate($42_Test_R_$memory, $t0, $DereferenceProphecy($t6));
+        $42_Test_R_$memoryPair := $MemoryPair ($42_Test_R_$Memory#1, $42_Test_R_$Memory, $t6->r_order);
+        //compute result
+        // assert forall addr: address: TypeDomain<address>() where exists[@1]<Test::R>(addr): exists<Test::R>(addr) at ./sources/FirstModule.move:7:9+82
+        // global invariant at ./sources/FirstModule.move:7:9+82
+        assume {:print "$at(2,107,189)"} true;
+        $tempresult := (forall addr: int :: $IsValid'address'(addr) ==> ($ResourceExistsMP($42_Test_R_$memoryPair, addr, $6->r_order - 1))  ==> ($ResourceExistsMP($42_Test_R_$memoryPair, addr, $6->r_order)));
+        if (!$tempresult && ($asserts_results || $t6->r_order < $asserts_time)) {
+            $assertType := 1;
+            $asserts_time := $t6->r_order;
+        }
+    }
+    if ($abort_flag) {
+        assume {:print "$at(2,289,306)"} true;
+        $t8 := $abort_code;
+        assume {:print "$track_abort(1,0):", $t8} $t8 == $t8;
+        goto L4;
+    }
 
-    // label L2 at ./sources/FirstModule.move:29:5+1
+    // $t4 := $t6 at ./sources/FirstModule.move:10:17+60
+    $t4 := $t6;
+
+    // fulfilled($t6) at ./sources/FirstModule.move:10:17+60
+    assume $Fulfilled($t6, $cur_index);
+    $cur_index := $cur_index + 1;
+
+    // goto L2 at ./sources/FirstModule.move:10:17+60
+    goto L2;
+
+    // label L0 at ./sources/FirstModule.move:10:75+1
+L0:
+
+    // $t7 := borrow_global<Test::R>($t0) on_abort goto L4 with $t8 at ./sources/FirstModule.move:10:54+17
+    assume {:print "$at(2,318,335)"} true;
+    if (!$ResourceExists($42_Test_R_$memory, $t0)) {
+        call $ExecFailureAbort();
+    } else {
+        call $t7 := $MutationAlt($Global($t0), EmptyVec(), $ResourceValue($42_Test_R_$memory, $t0));
+        //following line is not needed but acts as a sanity check. 
+        assume $ResourceValue($42_Test_R_$memory, $t0) == $Dereference($t7);
+        $42_Test_R_$memory#1 := $42_Test_R_$memory;
+        $42_Test_R_$memory := $ResourceUpdate($42_Test_R_$memory, $t0, $DereferenceProphecy($t7));
+        $42_Test_R_$memoryPair := $MemoryPair ($42_Test_R_$Memory#1, $42_Test_R_$Memory, $t6->r_order);
+        //compute result
+        // assert forall addr: address: TypeDomain<address>() where exists[@1]<Test::R>(addr): exists<Test::R>(addr) at ./sources/FirstModule.move:7:9+82
+        // global invariant at ./sources/FirstModule.move:7:9+82
+        assume {:print "$at(2,107,189)"} true;
+        $tempresult := (forall addr: int :: $IsValid'address'(addr) ==> ($ResourceExistsMP($42_Test_R_$memoryPair, addr, $7->r_order - 1))  ==> ($ResourceExistsMP($42_Test_R_$memoryPair, addr, $7->r_order)));
+        if (!$tempresult && ($asserts_results || $t7->r_order < $asserts_time)) {
+            $assertType := 1;
+            $asserts_time := $t7->r_order;
+        }
+    }
+    if ($abort_flag) {
+        assume {:print "$at(2,318,335)"} true;
+        $t8 := $abort_code;
+        assume {:print "$track_abort(1,0):", $t8} $t8 == $t8;
+        goto L4;
+    }
+
+    // $t4 := $t7 at ./sources/FirstModule.move:10:17+60
+    $t4 := $t7;
+
+    // fulfilled($t7) at ./sources/FirstModule.move:10:17+60
+    assume $Fulfilled($t7, $cur_index);
+    $cur_index := $cur_index + 1;
+
+    // label L2 at ./sources/FirstModule.move:10:17+60
 L2:
 
-    // abort($t5) at ./sources/FirstModule.move:29:5+1
-    assume {:print "$at(2,807,808)"} true;
-    $abort_code := $t5;
-    $abort_flag := true;
-    return;
+    // trace_local[c]($t4) at ./sources/FirstModule.move:10:13+1
+    assume {:print "$at(2,277,278)"} true;
+    $temp_0'$42_Test_R' := $Dereference($t4);
+    assume {:print "$track_local(1,0,5):", $temp_0'$42_Test_R'} $temp_0'$42_Test_R' == $temp_0'$42_Test_R';
 
-}
+    // $t9 := get_field<Test::R>.v1($t4) at ./sources/FirstModule.move:11:16+4
+    assume {:print "$at(2,358,362)"} true;
+    $t9 := $Dereference($t4)->$v1;
 
-// fun Test::incr2 [verification] at ./sources/FirstModule.move:30:5+265
-procedure {:timeLimit 80} $82_Test_incr2$verify(_$t0: int, _$t1: int) returns ()
-{
-    // declare local variables
-    var $t2: $Mutation ($82_Test_R);
-    var $t3: $Mutation ($82_Test_Y);
-    var $t4: $Mutation ($82_Test_R);
-    var $t5: int;
-    var $t6: $Mutation ($82_Test_Y);
-    var $t7: int;
-    var $t8: int;
-    var $t9: int;
-    var $t10: $Mutation (int);
-    var $t11: int;
-    var $t12: int;
-    var $t13: int;
-    var $t14: $Mutation (int);
-    var $t0: int;
-    var $t1: int;
-    var $temp_0'$82_Test_R': $82_Test_R;
-    var $temp_0'$82_Test_Y': $82_Test_Y;
-    var $temp_0'address': int;
-    $t0 := _$t0;
-    $t1 := _$t1;
+    // $t10 := 1 at ./sources/FirstModule.move:11:21+1
+    $t10 := 1;
+    assume $IsValid'u64'($t10);
 
-    // verification entrypoint assumptions
-    call $InitVerification();
-
-    // bytecode translation starts here
-    // assume WellFormed($t0) at ./sources/FirstModule.move:30:5+1
-    assume {:print "$at(2,813,814)"} true;
-    assume $IsValid'address'($t0);
-
-    // assume WellFormed($t1) at ./sources/FirstModule.move:30:5+1
-    assume $IsValid'address'($t1);
-
-    // assume forall $rsc: Test::R: ResourceDomain<Test::R>(): WellFormed($rsc) at ./sources/FirstModule.move:30:5+1
-    assume (forall $a_0: int :: {$ResourceValue($82_Test_R_$memory, $a_0)}(var $rsc := $ResourceValue($82_Test_R_$memory, $a_0);
-    ($IsValid'$82_Test_R'($rsc))));
-
-    // assume forall $rsc: Test::Y: ResourceDomain<Test::Y>(): WellFormed($rsc) at ./sources/FirstModule.move:30:5+1
-    assume (forall $a_0: int :: {$ResourceValue($82_Test_Y_$memory, $a_0)}(var $rsc := $ResourceValue($82_Test_Y_$memory, $a_0);
-    ($IsValid'$82_Test_Y'($rsc))));
-
-    // assume forall a: address: TypeDomain<address>() where exists<Test::R>(a): Eq<address>(a, 0x0) at ./sources/FirstModule.move:30:5+265
-    // global invariant at ./sources/FirstModule.move:10:9+70
-    assume (forall a: int :: $IsValid'address'(a) ==> ($ResourceExists($82_Test_R_$memory, a))  ==> ($IsEqual'address'(a, 0)));
-
-    // assume forall b: address: TypeDomain<address>() where exists<Test::Y>(b): Eq<address>(b, 0x30) at ./sources/FirstModule.move:30:5+265
-    // global invariant at ./sources/FirstModule.move:12:9+71
-    assume (forall b: int :: $IsValid'address'(b) ==> ($ResourceExists($82_Test_Y_$memory, b))  ==> ($IsEqual'address'(b, 48)));
-
-    // assume forall a: address: TypeDomain<address>() where exists<Test::R>(a): forall b: address: TypeDomain<address>() where exists<Test::Y>(b): Ge(select Test::R.x<Test::R>(global<Test::R>(a)), select Test::Y.x<Test::Y>(global<Test::Y>(b))) at ./sources/FirstModule.move:30:5+265
-    // global invariant at ./sources/FirstModule.move:14:9+147
-    assume (forall a: int :: $IsValid'address'(a) ==> ($ResourceExists($82_Test_R_$memory, a))  ==> ((forall b: int :: $IsValid'address'(b) ==> ($ResourceExists($82_Test_Y_$memory, b))  ==> (($ResourceValue($82_Test_R_$memory, a)->$x >= $ResourceValue($82_Test_Y_$memory, b)->$x)))));
-
-    // trace_local[a]($t0) at ./sources/FirstModule.move:30:5+1
-    assume {:print "$track_local(1,1,0):", $t0} $t0 == $t0;
-
-    // trace_local[b]($t1) at ./sources/FirstModule.move:30:5+1
-    assume {:print "$track_local(1,1,1):", $t1} $t1 == $t1;
-
-    // $t4 := borrow_global<Test::R>($t0) on_abort goto L2 with $t5 at ./sources/FirstModule.move:31:17+17
-    assume {:print "$at(2,884,901)"} true;
-    if (!$ResourceExists($82_Test_R_$memory, $t0)) {
-        call $ExecFailureAbort();
-    } else {
-        call $t4 := $MutationAlt($Global($t0), EmptyVec(), $ResourceValue($82_Test_R_$memory, $t0));
-        assume $ResourceValue($82_Test_R_$memory, $t0) == $Dereference($t4);
-        $82_Test_R_$memory := $ResourceUpdate($82_Test_R_$memory, $t0, $DereferenceProphecy($t4));
-    }
+    // $t11 := +($t9, $t10) on_abort goto L4 with $t8 at ./sources/FirstModule.move:11:20+1
+    call $t11 := $AddU64($t9, $t10);
     if ($abort_flag) {
-        assume {:print "$at(2,884,901)"} true;
-        $t5 := $abort_code;
-        assume {:print "$track_abort(1,1):", $t5} $t5 == $t5;
-        goto L2;
+        assume {:print "$at(2,362,363)"} true;
+        $t8 := $abort_code;
+        assume {:print "$track_abort(1,0):", $t8} $t8 == $t8;
+        goto L4;
     }
 
-    // trace_local[r]($t4) at ./sources/FirstModule.move:31:13+1
-    $temp_0'$82_Test_R' := $Dereference($t4);
-    assume {:print "$track_local(1,1,2):", $temp_0'$82_Test_R'} $temp_0'$82_Test_R' == $temp_0'$82_Test_R';
+    // $t12 := borrow_field<Test::R>.v1($t4) at ./sources/FirstModule.move:11:9+4
+    call $t12 := $ChildMutationAlt($t4, 0, $Dereference($t4)->$v1);
+    assume $Dereference($t12) == $Dereference($t4)->$v1;
+    $t4 := $UpdateMutationRToken($t4, $t12);
+    $t4 := $UpdateMutation($t4, $Update'$42_Test_R'_v1($Dereference($t4), $DereferenceProphecy($t12)));
 
-    // $t6 := borrow_global<Test::Y>($t1) on_abort goto L2 with $t5 at ./sources/FirstModule.move:32:18+17
-    assume {:print "$at(2,926,943)"} true;
-    if (!$ResourceExists($82_Test_Y_$memory, $t1)) {
-        call $ExecFailureAbort();
-    } else {
-        call $t6 := $MutationAlt($Global($t1), EmptyVec(), $ResourceValue($82_Test_Y_$memory, $t1));
-        assume $ResourceValue($82_Test_Y_$memory, $t1) == $Dereference($t6);
-        $82_Test_Y_$memory := $ResourceUpdate($82_Test_Y_$memory, $t1, $DereferenceProphecy($t6));
-    }
-    if ($abort_flag) {
-        assume {:print "$at(2,926,943)"} true;
-        $t5 := $abort_code;
-        assume {:print "$track_abort(1,1):", $t5} $t5 == $t5;
-        goto L2;
-    }
+    // fulfilled($t4) at ./sources/FirstModule.move:11:9+4
+    assume $Fulfilled($t4, $cur_index);
+    $cur_index := $cur_index + 1;
 
-    // trace_local[r2]($t6) at ./sources/FirstModule.move:32:13+2
-    $temp_0'$82_Test_Y' := $Dereference($t6);
-    assume {:print "$track_local(1,1,3):", $temp_0'$82_Test_Y'} $temp_0'$82_Test_Y' == $temp_0'$82_Test_Y';
+    // write_ref($t12, $t11) at ./sources/FirstModule.move:11:9+13
+    $t12 := $UpdateMutation($t12, $t11);
 
-    // $t7 := get_field<Test::R>.x($t4) at ./sources/FirstModule.move:33:15+3
-    assume {:print "$at(2,965,968)"} true;
-    $t7 := $Dereference($t4)->$x;
+    // write_back[Reference($t4).v1 (u64)]($t12) at ./sources/FirstModule.move:11:9+13
+    assume $Fulfilled($t12, $cur_index);
+    $cur_index := $cur_index + 1;
 
-    // $t8 := 1 at ./sources/FirstModule.move:33:21+1
-    $t8 := 1;
-    assume $IsValid'u64'($t8);
+    // trace_local[tmp#$4]($t4) at ./sources/FirstModule.move:11:9+13
+    $temp_0'$42_Test_R' := $Dereference($t4);
+    assume {:print "$track_local(1,0,4):", $temp_0'$42_Test_R'} $temp_0'$42_Test_R' == $temp_0'$42_Test_R';
 
-    // $t9 := +($t7, $t8) on_abort goto L2 with $t5 at ./sources/FirstModule.move:33:19+1
-    call $t9 := $AddU64($t7, $t8);
-    if ($abort_flag) {
-        assume {:print "$at(2,969,970)"} true;
-        $t5 := $abort_code;
-        assume {:print "$track_abort(1,1):", $t5} $t5 == $t5;
-        goto L2;
-    }
+    // write_back[Reference($t6)@]($t4) at ./sources/FirstModule.move:11:9+13
+    assume $Fulfilled($t4, $cur_index);
+    $cur_index := $cur_index + 1;
 
-    // $t10 := borrow_field<Test::R>.x($t4) at ./sources/FirstModule.move:33:9+3
-    call $t10 := $ChildMutationAlt($t4, 0, $Dereference($t4)->$x);
-    assume $Dereference($t10) == $Dereference($t4)->$x;
-    $t4 := $UpdateMutation($t4, $Update'$82_Test_R'_x($Dereference($t4), $DereferenceProphecy($t10)));
+    // @1 := save_mem(Test::R) at ./sources/FirstModule.move:9:5+171
+    // state save for global update invariants
+    assume {:print "$at(2,200,371)"} true;
+    $42_Test_R_$memory#1 := $42_Test_R_$memory;
 
-    // fulfilled($t4) at ./sources/FirstModule.move:33:9+3
-    assume $Fulfilled($t4);
-
-    // write_ref($t10, $t9) at ./sources/FirstModule.move:33:9+13
-    $t10 := $UpdateMutation($t10, $t9);
-
-    // write_back[Reference($t4).x (u64)]($t10) at ./sources/FirstModule.move:33:9+13
-    assume $Fulfilled($t10);
-
-    // write_back[Test::R@]($t4) at ./sources/FirstModule.move:33:9+13
-    assume $Dereference($t4) == $DereferenceProphecy($t4);
-
-    // assert forall a: address: TypeDomain<address>() where exists<Test::R>(a): Eq<address>(a, 0x0) at ./sources/FirstModule.move:10:9+70
-    // global invariant at ./sources/FirstModule.move:10:9+70
-    assume {:print "$at(2,137,207)"} true;
-    assert {:msg "assert_failed(2,137,207): global memory invariant does not hold"}
-      (forall a: int :: $IsValid'address'(a) ==> ($ResourceExists($82_Test_R_$memory, a))  ==> ($IsEqual'address'(a, 0)));
-
-    // assert forall a: address: TypeDomain<address>() where exists<Test::R>(a): forall b: address: TypeDomain<address>() where exists<Test::Y>(b): Ge(select Test::R.x<Test::R>(global<Test::R>(a)), select Test::Y.x<Test::Y>(global<Test::Y>(b))) at ./sources/FirstModule.move:14:9+147
-    // global invariant at ./sources/FirstModule.move:14:9+147
-    assume {:print "$at(2,296,443)"} true;
-    assert {:msg "assert_failed(2,296,443): global memory invariant does not hold"}
-      (forall a: int :: $IsValid'address'(a) ==> ($ResourceExists($82_Test_R_$memory, a))  ==> ((forall b: int :: $IsValid'address'(b) ==> ($ResourceExists($82_Test_Y_$memory, b))  ==> (($ResourceValue($82_Test_R_$memory, a)->$x >= $ResourceValue($82_Test_Y_$memory, b)->$x)))));
-
-    // $t11 := get_field<Test::Y>.x($t6) at ./sources/FirstModule.move:36:16+4
-    assume {:print "$at(2,1063,1067)"} true;
-    $t11 := $Dereference($t6)->$x;
-
-    // $t12 := 1 at ./sources/FirstModule.move:36:23+1
-    $t12 := 1;
-    assume $IsValid'u64'($t12);
-
-    // $t13 := +($t11, $t12) on_abort goto L2 with $t5 at ./sources/FirstModule.move:36:21+1
-    call $t13 := $AddU64($t11, $t12);
-    if ($abort_flag) {
-        assume {:print "$at(2,1068,1069)"} true;
-        $t5 := $abort_code;
-        assume {:print "$track_abort(1,1):", $t5} $t5 == $t5;
-        goto L2;
-    }
-
-    // $t14 := borrow_field<Test::Y>.x($t6) at ./sources/FirstModule.move:36:9+4
-    call $t14 := $ChildMutationAlt($t6, 0, $Dereference($t6)->$x);
-    assume $Dereference($t14) == $Dereference($t6)->$x;
-    $t6 := $UpdateMutation($t6, $Update'$82_Test_Y'_x($Dereference($t6), $DereferenceProphecy($t14)));
-
-    // fulfilled($t6) at ./sources/FirstModule.move:36:9+4
-    assume $Fulfilled($t6);
-
-    // write_ref($t14, $t13) at ./sources/FirstModule.move:36:9+15
-    $t14 := $UpdateMutation($t14, $t13);
-
-    // write_back[Reference($t6).x (u64)]($t14) at ./sources/FirstModule.move:36:9+15
-    assume $Fulfilled($t14);
-
-    // write_back[Test::Y@]($t6) at ./sources/FirstModule.move:36:9+15
+    // write_back[Test::R@]($t6) at ./sources/FirstModule.move:11:9+13
+    assume {:print "$at(2,351,364)"} true;
     assume $Dereference($t6) == $DereferenceProphecy($t6);
 
-    // assert forall b: address: TypeDomain<address>() where exists<Test::Y>(b): Eq<address>(b, 0x30) at ./sources/FirstModule.move:12:9+71
-    // global invariant at ./sources/FirstModule.move:12:9+71
-    assume {:print "$at(2,216,287)"} true;
-    assert {:msg "assert_failed(2,216,287): global memory invariant does not hold"}
-      (forall b: int :: $IsValid'address'(b) ==> ($ResourceExists($82_Test_Y_$memory, b))  ==> ($IsEqual'address'(b, 48)));
+    // assert forall addr: address: TypeDomain<address>() where exists[@1]<Test::R>(addr): exists<Test::R>(addr) at ./sources/FirstModule.move:7:9+82
+    // global invariant at ./sources/FirstModule.move:7:9+82
+    assume {:print "$at(2,107,189)"} true;
+    assert {:msg "assert_failed(2,107,189): global memory invariant does not hold"}
+      (forall addr: int :: $IsValid'address'(addr) ==> ($ResourceExists($42_Test_R_$memory#1, addr))  ==> ($ResourceExists($42_Test_R_$memory, addr)));
 
-    // assert forall a: address: TypeDomain<address>() where exists<Test::R>(a): forall b: address: TypeDomain<address>() where exists<Test::Y>(b): Ge(select Test::R.x<Test::R>(global<Test::R>(a)), select Test::Y.x<Test::Y>(global<Test::Y>(b))) at ./sources/FirstModule.move:14:9+147
-    // global invariant at ./sources/FirstModule.move:14:9+147
-    assume {:print "$at(2,296,443)"} true;
-    assert {:msg "assert_failed(2,296,443): global memory invariant does not hold"}
-      (forall a: int :: $IsValid'address'(a) ==> ($ResourceExists($82_Test_R_$memory, a))  ==> ((forall b: int :: $IsValid'address'(b) ==> ($ResourceExists($82_Test_Y_$memory, b))  ==> (($ResourceValue($82_Test_R_$memory, a)->$x >= $ResourceValue($82_Test_Y_$memory, b)->$x)))));
+    // write_back[Reference($t4).v1 (u64)]($t12) at ./sources/FirstModule.move:11:9+13
+    assume {:print "$at(2,351,364)"} true;
+    assume $Fulfilled($t12, $cur_index);
+    $cur_index := $cur_index + 1;
 
-    // label L1 at ./sources/FirstModule.move:37:5+1
-    assume {:print "$at(2,1077,1078)"} true;
-L1:
+    // trace_local[tmp#$4]($t4) at ./sources/FirstModule.move:11:9+13
+    $temp_0'$42_Test_R' := $Dereference($t4);
+    assume {:print "$track_local(1,0,4):", $temp_0'$42_Test_R'} $temp_0'$42_Test_R' == $temp_0'$42_Test_R';
 
-    // return () at ./sources/FirstModule.move:37:5+1
-    assume {:print "$at(2,1077,1078)"} true;
+    // write_back[Reference($t7)@]($t4) at ./sources/FirstModule.move:11:9+13
+    assume $Fulfilled($t4, $cur_index);
+    $cur_index := $cur_index + 1;
+
+    // @2 := save_mem(Test::R) at ./sources/FirstModule.move:7:9+82
+    // state save for global update invariants
+    assume {:print "$at(2,107,189)"} true;
+    $42_Test_R_$memory#2 := $42_Test_R_$memory;
+
+    // write_back[Test::R@]($t7) at ./sources/FirstModule.move:11:9+13
+    assume {:print "$at(2,351,364)"} true;
+    assume $Fullfilled($t7, $cur_index);
+    $cur_index := $cur_index + 1;
+
+    // label L3 at ./sources/FirstModule.move:12:5+1
+    assume {:print "$at(2,370,371)"} true;
+L3:
+
+    // return () at ./sources/FirstModule.move:12:5+1
+    if ($isEntryPoint){
+        var $i: int;
+        if($asserts_results){
+            if ($assertType == 1){
+                assert {:msg "assert_failed(2,107,189): global memory invariant does not hold"} false;
+            }
+        }
+    }
+    assume {:print "$at(2,370,371)"} true;
     return;
 
-    // label L2 at ./sources/FirstModule.move:37:5+1
-L2:
+    // label L4 at ./sources/FirstModule.move:12:5+1
+L4:
 
-    // abort($t5) at ./sources/FirstModule.move:37:5+1
-    assume {:print "$at(2,1077,1078)"} true;
-    $abort_code := $t5;
+    // abort($t8) at ./sources/FirstModule.move:12:5+1
+    assume {:print "$at(2,370,371)"} true;
+    $abort_code := $t8;
     $abort_flag := true;
     return;
 
-}
+    // label L5 at <internal>:1:1+10
+    assume {:print "$at(1,0,10)"} true;
+L5:
 
-// fun Test::incr3 [verification] at ./sources/FirstModule.move:38:5+191
-procedure {:timeLimit 80} $82_Test_incr3$verify(_$t0: int, _$t1: int) returns ()
-{
-    // declare local variables
-    var $t2: $Mutation ($82_Test_R);
-    var $t3: $Mutation ($82_Test_Y);
-    var $t4: $Mutation ($82_Test_Y);
-    var $t5: int;
-    var $t6: $Mutation ($82_Test_R);
-    var $t7: int;
-    var $t8: int;
-    var $t9: int;
-    var $t10: $Mutation (int);
-    var $t11: int;
-    var $t12: int;
-    var $t13: int;
-    var $t14: $Mutation (int);
-    var $t0: int;
-    var $t1: int;
-    var $temp_0'$82_Test_R': $82_Test_R;
-    var $temp_0'$82_Test_Y': $82_Test_Y;
-    var $temp_0'address': int;
-    $t0 := _$t0;
-    $t1 := _$t1;
+    // drop($t6) at <internal>:1:1+10
+    assume {:print "$at(1,0,10)"} true;
 
-    // verification entrypoint assumptions
-    call $InitVerification();
+    // goto L1 at <internal>:1:1+10
+    goto L1;
 
-    // bytecode translation starts here
-    // assume WellFormed($t0) at ./sources/FirstModule.move:38:5+1
-    assume {:print "$at(2,1083,1084)"} true;
-    assume $IsValid'address'($t0);
+    // label L6 at <internal>:1:1+10
+L6:
 
-    // assume WellFormed($t1) at ./sources/FirstModule.move:38:5+1
-    assume $IsValid'address'($t1);
+    // drop($t7) at <internal>:1:1+10
+    assume {:print "$at(1,0,10)"} true;
 
-    // assume forall $rsc: Test::R: ResourceDomain<Test::R>(): WellFormed($rsc) at ./sources/FirstModule.move:38:5+1
-    assume (forall $a_0: int :: {$ResourceValue($82_Test_R_$memory, $a_0)}(var $rsc := $ResourceValue($82_Test_R_$memory, $a_0);
-    ($IsValid'$82_Test_R'($rsc))));
-
-    // assume forall $rsc: Test::Y: ResourceDomain<Test::Y>(): WellFormed($rsc) at ./sources/FirstModule.move:38:5+1
-    assume (forall $a_0: int :: {$ResourceValue($82_Test_Y_$memory, $a_0)}(var $rsc := $ResourceValue($82_Test_Y_$memory, $a_0);
-    ($IsValid'$82_Test_Y'($rsc))));
-
-    // assume forall a: address: TypeDomain<address>() where exists<Test::R>(a): Eq<address>(a, 0x0) at ./sources/FirstModule.move:38:5+191
-    // global invariant at ./sources/FirstModule.move:10:9+70
-    assume (forall a: int :: $IsValid'address'(a) ==> ($ResourceExists($82_Test_R_$memory, a))  ==> ($IsEqual'address'(a, 0)));
-
-    // assume forall b: address: TypeDomain<address>() where exists<Test::Y>(b): Eq<address>(b, 0x30) at ./sources/FirstModule.move:38:5+191
-    // global invariant at ./sources/FirstModule.move:12:9+71
-    assume (forall b: int :: $IsValid'address'(b) ==> ($ResourceExists($82_Test_Y_$memory, b))  ==> ($IsEqual'address'(b, 48)));
-
-    // assume forall a: address: TypeDomain<address>() where exists<Test::R>(a): forall b: address: TypeDomain<address>() where exists<Test::Y>(b): Ge(select Test::R.x<Test::R>(global<Test::R>(a)), select Test::Y.x<Test::Y>(global<Test::Y>(b))) at ./sources/FirstModule.move:38:5+191
-    // global invariant at ./sources/FirstModule.move:14:9+147
-    assume (forall a: int :: $IsValid'address'(a) ==> ($ResourceExists($82_Test_R_$memory, a))  ==> ((forall b: int :: $IsValid'address'(b) ==> ($ResourceExists($82_Test_Y_$memory, b))  ==> (($ResourceValue($82_Test_R_$memory, a)->$x >= $ResourceValue($82_Test_Y_$memory, b)->$x)))));
-
-    // trace_local[a]($t0) at ./sources/FirstModule.move:38:5+1
-    assume {:print "$track_local(1,2,0):", $t0} $t0 == $t0;
-
-    // trace_local[b]($t1) at ./sources/FirstModule.move:38:5+1
-    assume {:print "$track_local(1,2,1):", $t1} $t1 == $t1;
-
-    // $t4 := borrow_global<Test::Y>($t1) on_abort goto L2 with $t5 at ./sources/FirstModule.move:39:18+17
-    assume {:print "$at(2,1155,1172)"} true;
-    if (!$ResourceExists($82_Test_Y_$memory, $t1)) {
-        call $ExecFailureAbort();
-    } else {
-        call $t4 := $MutationAlt($Global($t1), EmptyVec(), $ResourceValue($82_Test_Y_$memory, $t1));
-        assume $ResourceValue($82_Test_Y_$memory, $t1) == $Dereference($t4);
-        $82_Test_Y_$memory := $ResourceUpdate($82_Test_Y_$memory, $t1, $DereferenceProphecy($t4));
-    }
-    if ($abort_flag) {
-        assume {:print "$at(2,1155,1172)"} true;
-        $t5 := $abort_code;
-        assume {:print "$track_abort(1,2):", $t5} $t5 == $t5;
-        goto L2;
-    }
-
-    // trace_local[r2]($t4) at ./sources/FirstModule.move:39:13+2
-    $temp_0'$82_Test_Y' := $Dereference($t4);
-    assume {:print "$track_local(1,2,3):", $temp_0'$82_Test_Y'} $temp_0'$82_Test_Y' == $temp_0'$82_Test_Y';
-
-    // $t6 := borrow_global<Test::R>($t0) on_abort goto L2 with $t5 at ./sources/FirstModule.move:40:17+17
-    assume {:print "$at(2,1196,1213)"} true;
-    if (!$ResourceExists($82_Test_R_$memory, $t0)) {
-        call $ExecFailureAbort();
-    } else {
-        call $t6 := $MutationAlt($Global($t0), EmptyVec(), $ResourceValue($82_Test_R_$memory, $t0));
-        assume $ResourceValue($82_Test_R_$memory, $t0) == $Dereference($t6);
-        $82_Test_R_$memory := $ResourceUpdate($82_Test_R_$memory, $t0, $DereferenceProphecy($t6));
-    }
-    if ($abort_flag) {
-        assume {:print "$at(2,1196,1213)"} true;
-        $t5 := $abort_code;
-        assume {:print "$track_abort(1,2):", $t5} $t5 == $t5;
-        goto L2;
-    }
-
-    // trace_local[r]($t6) at ./sources/FirstModule.move:40:13+1
-    $temp_0'$82_Test_R' := $Dereference($t6);
-    assume {:print "$track_local(1,2,2):", $temp_0'$82_Test_R'} $temp_0'$82_Test_R' == $temp_0'$82_Test_R';
-
-    // $t7 := get_field<Test::R>.x($t6) at ./sources/FirstModule.move:41:15+3
-    assume {:print "$at(2,1235,1238)"} true;
-    $t7 := $Dereference($t6)->$x;
-
-    // $t8 := 1 at ./sources/FirstModule.move:41:21+1
-    $t8 := 1;
-    assume $IsValid'u64'($t8);
-
-    // $t9 := +($t7, $t8) on_abort goto L2 with $t5 at ./sources/FirstModule.move:41:19+1
-    call $t9 := $AddU64($t7, $t8);
-    if ($abort_flag) {
-        assume {:print "$at(2,1239,1240)"} true;
-        $t5 := $abort_code;
-        assume {:print "$track_abort(1,2):", $t5} $t5 == $t5;
-        goto L2;
-    }
-
-    // $t10 := borrow_field<Test::R>.x($t6) at ./sources/FirstModule.move:41:9+3
-    call $t10 := $ChildMutationAlt($t6, 0, $Dereference($t6)->$x);
-    assume $Dereference($t10) == $Dereference($t6)->$x;
-    $t6 := $UpdateMutation($t6, $Update'$82_Test_R'_x($Dereference($t6), $DereferenceProphecy($t10)));
-
-    // fulfilled($t6) at ./sources/FirstModule.move:41:9+3
-    assume $Fulfilled($t6);
-
-    // write_ref($t10, $t9) at ./sources/FirstModule.move:41:9+13
-    $t10 := $UpdateMutation($t10, $t9);
-
-    // write_back[Reference($t6).x (u64)]($t10) at ./sources/FirstModule.move:41:9+13
-    assume $Fulfilled($t10);
-
-    // write_back[Test::R@]($t6) at ./sources/FirstModule.move:41:9+13
-    assume $Dereference($t6) == $DereferenceProphecy($t6);
-
-    // assert forall a: address: TypeDomain<address>() where exists<Test::R>(a): Eq<address>(a, 0x0) at ./sources/FirstModule.move:10:9+70
-    // global invariant at ./sources/FirstModule.move:10:9+70
-    assume {:print "$at(2,137,207)"} true;
-    assert {:msg "assert_failed(2,137,207): global memory invariant does not hold"}
-      (forall a: int :: $IsValid'address'(a) ==> ($ResourceExists($82_Test_R_$memory, a))  ==> ($IsEqual'address'(a, 0)));
-
-    // assert forall a: address: TypeDomain<address>() where exists<Test::R>(a): forall b: address: TypeDomain<address>() where exists<Test::Y>(b): Ge(select Test::R.x<Test::R>(global<Test::R>(a)), select Test::Y.x<Test::Y>(global<Test::Y>(b))) at ./sources/FirstModule.move:14:9+147
-    // global invariant at ./sources/FirstModule.move:14:9+147
-    assume {:print "$at(2,296,443)"} true;
-    assert {:msg "assert_failed(2,296,443): global memory invariant does not hold"}
-      (forall a: int :: $IsValid'address'(a) ==> ($ResourceExists($82_Test_R_$memory, a))  ==> ((forall b: int :: $IsValid'address'(b) ==> ($ResourceExists($82_Test_Y_$memory, b))  ==> (($ResourceValue($82_Test_R_$memory, a)->$x >= $ResourceValue($82_Test_Y_$memory, b)->$x)))));
-
-    // $t11 := get_field<Test::Y>.x($t4) at ./sources/FirstModule.move:42:16+4
-    assume {:print "$at(2,1259,1263)"} true;
-    $t11 := $Dereference($t4)->$x;
-
-    // $t12 := 1 at ./sources/FirstModule.move:42:23+1
-    $t12 := 1;
-    assume $IsValid'u64'($t12);
-
-    // $t13 := +($t11, $t12) on_abort goto L2 with $t5 at ./sources/FirstModule.move:42:21+1
-    call $t13 := $AddU64($t11, $t12);
-    if ($abort_flag) {
-        assume {:print "$at(2,1264,1265)"} true;
-        $t5 := $abort_code;
-        assume {:print "$track_abort(1,2):", $t5} $t5 == $t5;
-        goto L2;
-    }
-
-    // $t14 := borrow_field<Test::Y>.x($t4) at ./sources/FirstModule.move:42:9+4
-    call $t14 := $ChildMutationAlt($t4, 0, $Dereference($t4)->$x);
-    assume $Dereference($t14) == $Dereference($t4)->$x;
-    $t4 := $UpdateMutation($t4, $Update'$82_Test_Y'_x($Dereference($t4), $DereferenceProphecy($t14)));
-
-    // fulfilled($t4) at ./sources/FirstModule.move:42:9+4
-    assume $Fulfilled($t4);
-
-    // write_ref($t14, $t13) at ./sources/FirstModule.move:42:9+15
-    $t14 := $UpdateMutation($t14, $t13);
-
-    // write_back[Reference($t4).x (u64)]($t14) at ./sources/FirstModule.move:42:9+15
-    assume $Fulfilled($t14);
-
-    // write_back[Test::Y@]($t4) at ./sources/FirstModule.move:42:9+15
-    assume $Dereference($t4) == $DereferenceProphecy($t4);
-
-    // assert forall b: address: TypeDomain<address>() where exists<Test::Y>(b): Eq<address>(b, 0x30) at ./sources/FirstModule.move:12:9+71
-    // global invariant at ./sources/FirstModule.move:12:9+71
-    assume {:print "$at(2,216,287)"} true;
-    assert {:msg "assert_failed(2,216,287): global memory invariant does not hold"}
-      (forall b: int :: $IsValid'address'(b) ==> ($ResourceExists($82_Test_Y_$memory, b))  ==> ($IsEqual'address'(b, 48)));
-
-    // assert forall a: address: TypeDomain<address>() where exists<Test::R>(a): forall b: address: TypeDomain<address>() where exists<Test::Y>(b): Ge(select Test::R.x<Test::R>(global<Test::R>(a)), select Test::Y.x<Test::Y>(global<Test::Y>(b))) at ./sources/FirstModule.move:14:9+147
-    // global invariant at ./sources/FirstModule.move:14:9+147
-    assume {:print "$at(2,296,443)"} true;
-    assert {:msg "assert_failed(2,296,443): global memory invariant does not hold"}
-      (forall a: int :: $IsValid'address'(a) ==> ($ResourceExists($82_Test_R_$memory, a))  ==> ((forall b: int :: $IsValid'address'(b) ==> ($ResourceExists($82_Test_Y_$memory, b))  ==> (($ResourceValue($82_Test_R_$memory, a)->$x >= $ResourceValue($82_Test_Y_$memory, b)->$x)))));
-
-    // label L1 at ./sources/FirstModule.move:43:5+1
-    assume {:print "$at(2,1273,1274)"} true;
-L1:
-
-    // return () at ./sources/FirstModule.move:43:5+1
-    assume {:print "$at(2,1273,1274)"} true;
-    return;
-
-    // label L2 at ./sources/FirstModule.move:43:5+1
-L2:
-
-    // abort($t5) at ./sources/FirstModule.move:43:5+1
-    assume {:print "$at(2,1273,1274)"} true;
-    $abort_code := $t5;
-    $abort_flag := true;
-    return;
+    // goto L0 at <internal>:1:1+10
+    goto L0;
 
 }
